Various updates/improvements to the decompiler tools.

examples/l3-machine-code/arm/decompiler/arm_core_decompLib.sig
@@ -1,8 +1,4 @@
 signature arm_core_decompLib =
 sig
-
-    val l3_triple: string -> (Thm.thm * int * int option) *
-                             (Thm.thm * int * int option) option
-    val swap_primes: Term.term -> Term.term
-
+    val l3_triple: string -> helperLib.instruction
 end
