examples/l3-machine-code/arm/decompiler/arm_decompLib.sig
@@ -1,9 +1,13 @@
 signature arm_decompLib =
 sig
 
-    val config_for_fast   : unit -> unit
-    val l3_arm_triples    : string -> Thm.thm list
-    val l3_arm_tools      : helperLib.decompiler_tools
-    val l3_arm_decompile  : string -> Term.term quotation -> Thm.thm * Thm.thm
+    val config_for_fast: unit -> unit
+    val config_for_original: unit -> unit
+    val l3_arm_decompile: string -> Term.term quotation -> Thm.thm * Thm.thm
+    val l3_arm_decompile_no_status:
+       string -> Term.term quotation -> Thm.thm * Thm.thm
+    val l3_arm_tools: helperLib.decompiler_tools
+    val l3_arm_tools_no_status: helperLib.decompiler_tools
+    val l3_arm_triples: string -> Thm.thm list
 
 end
