examples/l3-machine-code/arm/prog/arm_progLib.sig
@@ -6,8 +6,5 @@ sig
    val arm_spec: string -> Thm.thm list
    val arm_spec_hex: string -> Thm.thm list
 
-   val loadSpecs: Thm.thm -> unit
-   val saveSpecs: string -> Thm.thm
-
    val set_newline: string -> unit
 end
