examples/l3-machine-code/common/core_decompilerLib.sig
@@ -3,8 +3,9 @@ sig
 
    val configure: {pc_tm: Term.term,
                    init_fn: unit -> unit,
+                   pc_conv: Conv.conv -> Conv.conv,
                    triple_fn: string -> helperLib.instruction,
-                   swap_fn: Term.term -> Term.term} -> unit
+                   component_vars: Term.term list} -> unit
 
    val core_decompile: string -> Term.term quotation -> Thm.thm * Thm.thm
 
