examples/l3-machine-code/common/core_decompilerLib.sml
@@ -3,6 +3,7 @@ struct
 
 open HolKernel Parse boolLib bossLib
 open helperLib tripleTheory
+open tripleSyntax
 
 val ERR = Feedback.mk_HOL_ERR "core_decompilerLib"
 
@@ -20,17 +21,28 @@ val ERR = Feedback.mk_HOL_ERR "core_decompilerLib"
 val get_triple =
    ref (fn _: string =>
           (raise ERR "get_triple" "uninitialised"): helperLib.instruction)
-val initialise = ref (fn () => ())
-val swap_primes = ref (Lib.I: term -> term)
+val initialise = ref (Lib.I: unit -> unit)
 val pc = ref boolSyntax.F
 val pc_size = ref 0
+val at_pc_conv = ref (Lib.I: conv -> conv)
+val swap_primes = ref (Lib.I: term -> term)
 
-fun configure {triple_fn = f, init_fn = i, swap_fn = s, pc_tm = p} =
+fun add_prime v = Term.mk_var (fst (Term.dest_var v) ^ "'", Term.type_of v)
+
+fun configure
+   {triple_fn = f, init_fn = i, pc_tm = p, pc_conv = c, component_vars = vs} =
    ( get_triple := f
      ; initialise := i
-     ; swap_primes := s
      ; pc := p
-     ; pc_size := Arbnum.toInt (wordsSyntax.size_of p) )
+     ; at_pc_conv := c
+     ; pc_size := Arbnum.toInt (wordsSyntax.size_of p)
+     ; swap_primes :=
+         Term.subst
+            (List.concat
+               (List.map
+                  (fn v =>
+                     let val pv = add_prime v in [v |-> pv, pv |-> v] end) vs))
+   )
 
 val code_abbrevs = ref ([]:thm list);
 fun add_code_abbrev th = (code_abbrevs := th::(!code_abbrevs));
@@ -39,38 +51,6 @@ val decomp_mem = ref ([]:(string * thm * int) list);
 fun add_decomp name th len = (decomp_mem := ((name,th,len)::(!decomp_mem)));
 
 (* PHASE 1 -- evaluate model *)
-
-val strip_string = Substring.string o Substring.dropr Char.isSpace o
-                   Substring.dropl Char.isSpace o Substring.full
-
-(* Turns a quote `...` into a list of strings *)
-local
-   fun get_QUOTE (QUOTE t) = t | get_QUOTE _ = fail()
-   fun strip_comments l [] = []
-     | strip_comments l [x] = if 0 < l then [] else [x]
-     | strip_comments l (x::y::xs) =
-         if x = #"(" andalso y = #"*"
-            then strip_comments (l + 1) xs
-         else if x = #"*" andalso y = #")"
-            then strip_comments (l - 1) xs
-         else if 0 < l
-            then strip_comments l (y::xs)
-         else x :: strip_comments l (y::xs)
-   fun lines [] [] = []
-     | lines xs [] = [implode (rev xs)]
-     | lines xs (y::ys) =
-         if mem y [#"\n", #"|"]
-            then implode (rev xs) :: lines [] ys
-         else lines (y::xs) ys
-in
-   fun quote_to_strings (q: term quotation) =
-      let
-         val xs = explode (get_QUOTE (hd q))
-         val zs = lines [] (strip_comments 0 xs)
-      in
-         filter (not o Lib.equal "") (map strip_string zs)
-      end
-end
 
 fun add_to_pc n =
    [!pc |-> wordsSyntax.mk_word_add (!pc, wordsSyntax.mk_wordii (n, !pc_size))]
@@ -93,29 +73,17 @@ local
       case Lib.total wordsSyntax.dest_word_add tm of
          SOME (v, _) => not (Term.is_var v)
        | _ => not (boolSyntax.is_cond tm)
-   (* val CODE_CONV = RATOR_CONV o RAND_CONV
-   val CODE_PC_CONV =
-      Conv.DEPTH_CONV
-         (fn tm =>
-            case Lib.total pairSyntax.dest_pair tm of
-              SOME (l, _) =>
-                 if is_reducible l
-                    then Conv.LAND_CONV ARITH_SUB_CONV tm
-                 else raise ERR "CODE_PC_CONV" ""
-             | _ => raise ERR "CODE_PC_CONV" "") *)
-   fun PC_CONV tm = if is_reducible tm then ARITH_SUB_CONV tm else ALL_CONV tm
-   val AT_PC_CONV = funpow 28 RATOR_CONV o RAND_CONV
-   val PC_CONV = AT_PC_CONV PC_CONV
-   val PC_RULE = Conv.CONV_RULE (PRE_ASSERT PC_CONV
-                                 (* THENC CODE_CONV CODE_PC_CONV *)
-                                 THENC POST_ASSERT PC_CONV)
+   fun PC_CONV tm =
+      if is_reducible tm then (!at_pc_conv) ARITH_SUB_CONV tm else ALL_CONV tm
+   val PC_RULE = Conv.CONV_RULE (PRE_ASSERT PC_CONV THENC POST_ASSERT PC_CONV)
    fun set_pc n (th, l, j) =
       (PC_RULE (Thm.INST (add_to_pc n) th), l, Option.map (fn i => n + i) j)
    fun derive1 hex n =
       if String.isPrefix "insert:" hex
          then let
                  val name =
-                    strip_string (String.extract (hex, size ("insert:"), NONE))
+                    helperLib.remove_whitespace
+                       (String.extract (hex, size ("insert:"), NONE))
                  val (_, th, l) = first (fn (n, _, _) => n = name) (!decomp_mem)
               in
                  (n + l, (set_pc n (UNDISCH_ALL th, l, SOME l), NONE))
@@ -147,14 +115,7 @@ in
       end
 end
 
-val model = rand o rator o rator o rator
-
 local
-   fun extract_code (_, ((th, _, _), _)) = th |> concl |> rator |> rand
-   fun triple_apply f (y, ((th1, x1, x2), NONE) : helperLib.instruction) =
-          (y, ((f th1, x1, x2), NONE))
-     | triple_apply f (y, ((th1, x1, x2), SOME (th2, y1, y2))) =
-          (y, ((f th1, x1, x2), SOME (f th2, y1, y2)))
    val tac =
       SIMP_TAC (srw_ss()) [pred_setTheory.SUBSET_DEF, pred_setTheory.UNION_DEF]
    val IN_DEFN = Q.prove(`(c = b) ==> a IN b ==> a IN c`, tac)
@@ -175,19 +136,19 @@ local
       HolKernel.list_mk_lbinop (Lib.curry pred_setSyntax.mk_union)
    val strip_union = HolKernel.strip_binop (Lib.total pred_setSyntax.dest_union)
    val get_model_name =
-      helperLib.to_lower o fst o Term.dest_const o model o Thm.concl
+      helperLib.to_lower o fst o Term.dest_const o tripleSyntax.dest_model o
+      Thm.concl
+   fun extract_code (_, ((th, _, _), _)) = tripleSyntax.dest_code (Thm.concl th)
    val get_code =
       (((Lib.mk_set o List.concat o List.map pred_setSyntax.strip_set) ##
         Lib.mk_set) o
        List.partition pred_setSyntax.is_insert o
        List.concat o List.map (strip_union o extract_code)):
        (int * helperLib.instruction) list -> term list * term list
-   val (conj1, conj2) =
-      case CONJUNCTS (SPEC_ALL boolTheory.OR_CLAUSES) of
-         c1 :: c2 :: _ => (c1, c2)
+   val (CONJ1_CONV, CONJ2_CONV) =
+      case Drule.CONJUNCTS (Drule.SPEC_ALL boolTheory.OR_CLAUSES) of
+         c1 :: c2 :: _ => (Conv.REWR_CONV c1, Conv.REWR_CONV c2)
        | _ => fail()
-   val CONJ1_CONV = Conv.REWR_CONV conj1
-   val CONJ2_CONV = Conv.REWR_CONV conj2
 in
    fun abbreviate_code _ [] = raise ERR "abbreviate_code" "no code"
      | abbreviate_code name (thms as (_: int, ((th, _, _), _)) :: _) =
@@ -221,7 +182,7 @@ in
                (def_name ^ "_def", boolSyntax.mk_eq (Term.mk_comb (v, x), cs))
          val () = add_code_abbrev code_def
          val spec_code_def = Drule.SPEC_ALL code_def
-         val tm = (fst o boolSyntax.dest_eq o Thm.concl) spec_code_def
+         val tm = boolSyntax.lhs (Thm.concl spec_code_def)
          val sty = Term.type_of cs
          val ty = pred_setSyntax.dest_set_type sty
          val inst_ty = Thm.INST_TYPE [Type.alpha |-> ty]
@@ -277,14 +238,14 @@ in
          val rule = CONV_RULE (subset_conv (rwts1 @ rwts2)) o
                     Thm.SPEC tm o MATCH_MP TRIPLE_EXTEND
       in
-         List.map (triple_apply rule) thms
+         List.map (fn (i, x) => (i, helperLib.instruction_apply rule x)) thms
       end
 end
 
 fun stage_1 name qcode =
    let
       val () = (!initialise) ()
-      val code = quote_to_strings qcode
+      val code = helperLib.quote_to_strings qcode
       val thms = derive_specs name code
    in
       abbreviate_code name thms
@@ -303,7 +264,7 @@ val (_, ((th, _, _), _)) = hd thms
 
 val extract_graph =
    List.concat o
-   List.map (fn (i: int, (((_, _, j), NONE): helperLib.instruction)) => [(i, j)]
+   List.map (fn (i, ((_, _, j), NONE): helperLib.instruction) => [(i: int, j)]
               | (i, ((_, _, j), SOME (_, _, k))) => [(i, j), (i, k)])
 
 val jumps2edges =
@@ -314,94 +275,141 @@ val jumps2edges =
 val all_distinct = Lib.mk_set
 
 fun drop_until P [] = []
-  | drop_until P (x::xs) = if P x then x::xs else drop_until P xs
+  | drop_until P (x :: xs) = if P x then x :: xs else drop_until P xs
 
 fun subset [] ys = true
-  | subset (x::xs) ys = mem x ys andalso subset xs ys
+  | subset (x :: xs) ys = mem x ys andalso subset xs ys
 
-fun extract_loops jumps = let
-  (* find all possible paths *)
-  val edges = jumps2edges jumps
-  fun all_paths_from edges i prefix = let
-    fun f [] = []
-      | f ((k,j)::xs) = if i = k then j :: f xs else f xs
-    val next = all_distinct (f edges)
-    val prefix = prefix @ [i]
-    val xs = map (fn x => if mem x prefix then [prefix @ [x]] else
-                          all_paths_from edges x prefix) next
-    val xs = if xs = [] then [[prefix]] else xs
-    in Lib.flatten xs end
-  val paths = all_paths_from edges 0 []
-  (* get looping points *)
-  fun is_loop xs = mem (last xs) (butlast xs)
-  val loops = all_distinct (map last (filter is_loop paths))
-  (* find loop bodies and tails *)
-  fun loop_body_tail i = let
-    val bodies = filter (fn xs => last xs = i) paths
-    val bodies = filter is_loop bodies
-    val bodies = map (drop_until (fn x => x = i) o butlast) bodies
-    val bodies = all_distinct (Lib.flatten bodies)
-    val tails = filter (fn xs => mem i xs andalso not (last xs = i)) paths
-    val tails = map (drop_until (fn x => x = i)) tails
-    in (i,bodies,tails) end
-  val summaries = map loop_body_tail loops
-  (* clean loop tails *)
-  fun clean_tails (i,xs,tails) = let
-    val tails = map (drop_until (fn x => not (mem x xs))) tails
-    val tails = filter (fn xs => not (xs = [])) tails
-    in (i,xs,tails) end
-  val zs = map clean_tails summaries
-  (* merge combined loops *)
-  val zs = map (fn (x,y,z) => ([x],y,z)) zs
-  fun find_and_merge zs = let
-    val ls = Lib.flatten (map (fn (x,y,z) => x) zs)
-    val qs = map (fn (x,y,z) => (x,y,map hd z)) zs
-    fun f ys = filter (fn x => mem x ls andalso (not (mem x ys)))
-    val qs = map (fn (x,y,z) => (x,all_distinct (f x y @ f x z))) qs
-    fun cross [] ys = []
-      | cross (x::xs) ys = map (fn y => (x,y)) ys @ cross xs ys
-    val edges = Lib.flatten (map (fn (x,y) => cross x y) qs)
-    val paths = map (fn i => all_paths_from edges i []) ls
-    val goals = map (fn (x,y) => (y,x)) edges
-    fun sat_goal ((i,j),path) = (hd path = i) andalso (mem j (tl path))
-    val (i,j) = fst (hd (filter sat_goal (cross goals (Lib.flatten paths))))
-    val (p1,q1,x1) = hd (filter (fn (x,y,z) => mem i x) zs)
-    val (p2,q2,x2) = hd (filter (fn (x,y,z) => mem j x) zs)
-    val (p,q,x) = (p1 @ p2, all_distinct (q1 @ q2), x1 @ x2)
-    val zs = (p,q,x) :: filter (fn (x,y,z) => not (mem i x) andalso not (mem j x)) zs
-    val zs = map clean_tails zs
-    in zs end
-  val zs = repeat find_and_merge zs
-  (* attempt to find common exit point *)
-  fun mem_all x [] = true
-    | mem_all x (xs::xss) = mem x xs andalso mem_all x xss
-  fun find_exit_points (x,y,z) = let
-    val q = hd (filter (fn x => mem_all x (tl z)) (hd z))
-    in (x,[q]) end handle Empty => (x,all_distinct (map hd z))
-  val zs = map find_exit_points zs
-  (* finalise *)
-  val exit = (all_distinct o map last o filter (not o is_loop)) paths
-  val zero = ([0],exit)
-  val zs = if filter (fn (x,y) => mem 0 x andalso subset exit y) zs = [] then zs @ [zero] else zs
-  fun list_before x y [] = true
-    | list_before x y (z::zs) = if z = y then false else
-                                if z = x then true else list_before x y zs
-  fun compare (xs,_) (ys,_) = let
-    val x = hd xs
-    val y = hd ys
-    val p = hd (filter (fn xs => mem x xs andalso mem y xs) paths)
-    in not (list_before x y p) end handle Empty => false
-  val loops = sort compare zs
-  (* sort internal  *)
-  val int_sort = sort (fn x => fn (y:int) => x <= y)
-  val loops = map (fn (xs,ys) => (int_sort xs, int_sort ys)) loops
-  in loops end;
+local
+   fun all_paths_from edges i prefix =
+      let
+         fun f [] = []
+           | f ((k, j) :: xs) = if i = k then j :: f xs else f xs
+        val next = all_distinct (f edges)
+        val prefix = prefix @ [i]
+        val xs = map (fn x => if mem x prefix
+                                 then [prefix @ [x]]
+                              else all_paths_from edges x prefix) next
+        val xs = if xs = [] then [[prefix]] else xs
+      in
+         Lib.flatten xs
+      end
 
-fun forks [] = []
-  | forks ((x1, y1)::xs) =
-       if can (first (fn (x2, _) => x1 = x2)) xs
-          then x1 :: (forks (filter (fn (x2, _) => x2 <> x1) xs))
-       else forks xs
+   fun is_loop xs = Lib.mem (List.last xs) (Lib.butlast xs)
+
+   (* clean loop tails *)
+   fun clean_tails (i, xs, tails) =
+      (i, xs,
+       List.mapPartial
+          (fn t => let
+                      val l = drop_until (fn x => not (mem x xs)) t
+                   in
+                      if List.null l then NONE else SOME l
+                   end) tails)
+
+   fun cross [] ys = []
+     | cross (x :: xs) ys = map (fn y => (x, y)) ys @ cross xs ys
+
+   fun sat_goal ((i, j), path) = hd path = i andalso mem j (tl path)
+
+   fun find_and_merge zs =
+      let
+         val ls = Lib.flatten (map (fn (x, y, z) => x) zs)
+         val qs = map (fn (x, y, z) => (x, y, map hd z)) zs
+         fun f ys = filter (fn x => mem x ls andalso (not (mem x ys)))
+         val qs = map (fn (x, y, z) => (x, all_distinct (f x y @ f x z))) qs
+         val edges = Lib.flatten (map (fn (x,y) => cross x y) qs)
+         val paths = map (fn i => all_paths_from edges i []) ls
+         val goals = map (fn (x,y) => (y,x)) edges
+         val (i, j) =
+            fst (hd (filter sat_goal (cross goals (Lib.flatten paths))))
+         val (p1, q1, x1) = hd (filter (fn (x,y,z) => mem i x) zs)
+         val (p2, q2, x2) = hd (filter (fn (x,y,z) => mem j x) zs)
+         val (p, q, x) = (p1 @ p2, all_distinct (q1 @ q2), x1 @ x2)
+         val zs =
+            (p,q,x) ::
+            filter (fn (x, y, z) => not (mem i x) andalso not (mem j x)) zs
+         val zs = map clean_tails zs
+      in
+         zs
+      end
+
+   fun mem_all x = List.all (Lib.mem x)
+
+   fun find_exit_points (x, y, z) =
+      let
+         val q = hd (filter (fn x => mem_all x (tl z)) (hd z))
+      in
+         (x, [q])
+      end
+      handle Empty => (x, all_distinct (map hd z))
+
+   fun list_before x y [] = true
+     | list_before x y (z :: zs) =
+           z <> y andalso (z = x orelse list_before x y zs)
+
+   val int_sort = Lib.sort (Lib.curry (op Int.<=))
+in
+   fun extract_loops jumps =
+      let
+         (* find all possible paths *)
+         val edges = jumps2edges jumps
+         val paths = all_paths_from edges 0 []
+         (* get looping points *)
+         val loops = all_distinct (map last (filter is_loop paths))
+         (* find loop bodies and tails *)
+         fun loop_body_tail i =
+            let
+               val bodies = filter (fn xs => last xs = i) paths
+               val bodies = filter is_loop bodies
+               val bodies = map (drop_until (fn x => x = i) o butlast) bodies
+               val bodies = all_distinct (Lib.flatten bodies)
+               val tails =
+                  filter (fn xs => mem i xs andalso not (last xs = i)) paths
+               val tails = map (drop_until (fn x => x = i)) tails
+            in
+               (fn (x, y, z) => ([x], y, z)) (clean_tails (i, bodies, tails))
+            end
+         val zs = map loop_body_tail loops
+         (* merge combined loops *)
+         val zs = repeat find_and_merge zs
+         (* attempt to find common exit point *)
+         val zs = map find_exit_points zs
+         (* finalise *)
+         val exit = (all_distinct o map last o filter (not o is_loop)) paths
+         val zero = ([0], exit)
+         val zs =
+            if List.null
+                 (filter (fn (x, y) => mem 0 x andalso subset exit y) zs)
+               then zs @ [zero]
+            else zs
+         fun compare (xs, _) (ys, _) =
+            let
+               val x = hd xs
+               val y = hd ys
+               val p = hd (filter (fn xs => mem x xs andalso mem y xs) paths)
+            in
+               not (list_before x y p)
+            end
+            handle Empty => false
+         val loops = sort compare zs
+         (* sort internal  *)
+         val loops = map (int_sort ## int_sort) loops
+      in
+         loops
+      end
+end
+
+local
+   fun forks_acc a =
+     fn [] => List.rev a
+      | (x1, _) :: xs =>
+          if List.exists (fn (x2, _) => x2 = x1) xs
+             then forks_acc (x1 :: a) (filter (fn (x2, _) => x2 <> x1) xs)
+          else forks_acc a xs
+in
+   val forks = forks_acc []
+end
 
 fun stage_12 name qcode =
    let
@@ -433,85 +441,85 @@ datatype compose_tree =
 
 fun is_rec (Repeat _) = true
   | is_rec (End _) = false
-  | is_rec (Cons (_,t)) = is_rec t
-  | is_rec (Merge (_,t1,t2)) = is_rec t1 orelse is_rec t2
-  | is_rec (ConsMerge (_,_,_,t)) = is_rec t
+  | is_rec (Cons (_, t)) = is_rec t
+  | is_rec (Merge (_, t1, t2)) = is_rec t1 orelse is_rec t2
+  | is_rec (ConsMerge (_, _, _, t)) = is_rec t
 
 local
    val find_Abbrev = find_term (can (match_term ``Abbrev b``))
 in
-   fun build_compose_tree (b,e) thms =
+   fun build_compose_tree (b, e) thms =
       let
          fun find_next i = first (fn (n, _:helperLib.instruction) => n = i) thms
-         fun sub init NONE = failwith("cannot handle bad exists")
+         fun sub init NONE =
+               raise ERR "build_compose_tree" "cannot handle bad exists"
            | sub init (SOME i) =
              if mem i e
                 then End i
              else if not init andalso mem i b
                 then Repeat i
              else case find_next i of
-                    (_, ((th1, l1, x1), NONE)) => Cons (th1, sub false x1)
-                  | (_, ((th1, l1, x1), SOME (th2, l2, x2))) =>
-                    if x1 = x2
-                       then let
-                               val t1 = sub false x1
-                               val tm = find_Abbrev (hd (hyp th1))
-                                        handle Empty => find_Abbrev (concl th1)
-                            in
-                               ConsMerge (rand tm, th1, th2, t1)
-                            end
-                    else let
-                            val t1 = Cons (th1,sub false x1)
-                            val t2 = Cons (th2,sub false x2)
-                            val tm = find_Abbrev (hd (hyp th1))
-                                     handle Empty => find_Abbrev (concl th1)
-                         in
-                            Merge (rand tm, t1, t2)
-                         end
+                     (_, ((th1, l1, x1), NONE)) => Cons (th1, sub false x1)
+                   | (_, ((th1, l1, x1), SOME (th2, l2, x2))) =>
+                     if x1 = x2
+                        then let
+                                val t1 = sub false x1
+                                val tm = find_Abbrev (hd (hyp th1))
+                                         handle Empty => find_Abbrev (concl th1)
+                             in
+                                ConsMerge (rand tm, th1, th2, t1)
+                             end
+                     else let
+                             val t1 = Cons (th1, sub false x1)
+                             val t2 = Cons (th2, sub false x2)
+                             val tm = find_Abbrev (hd (hyp th1))
+                                      handle Empty => find_Abbrev (concl th1)
+                          in
+                             Merge (rand tm, t1, t2)
+                          end
       in
          sub true (SOME (hd b))
       end
 end
 
-val l1 = ref TRUTH;
-val l2 = ref TRUTH;
+val l1 = ref TRUTH
+val l2 = ref TRUTH
 val l3 = ref T;
 
-fun VALUE_CONV c = RAND_CONV (RAND_CONV c)
-
-fun compose th1 th2 =
-   let
-      val th3 = MATCH_MP (MATCH_MP TRIPLE_COMPOSE_ALT th2) th1
-   in
-      if List.null (hyp th3)
-         then th3
-      else let
-              val tm = hd (hyp th3)
-              val lemma = SYM (ASSUME tm)
-              val (lhs, rhs) = dest_eq tm
-              val th4 =
-                 th3 |> CONV_RULE (VALUE_CONV (PairRules.UNPBETA_CONV rhs
-                                   THENC REWR_CONV (SYM (SPEC_ALL LET_THM))
-                                   THENC (RAND_CONV (fn _ => lemma))))
-              fun ii lhs rhs =
-                 let
-                    val (x,y) = pairSyntax.dest_pair rhs
-                    val x1 = pairSyntax.mk_fst lhs
-                    val y1 = pairSyntax.mk_snd lhs
-                 in
-                    (x |-> x1) :: ii y1 y
-                 end
-                 handle HOL_ERR _ => [rhs |-> lhs]
-              val th5 = INST (ii lhs rhs) (DISCH_ALL th4)
-                        |> CONV_RULE
-                             ((RATOR_CONV o RAND_CONV)
-                                 (PURE_REWRITE_CONV [pairTheory.PAIR]))
-                        |> (fn th => MP th (REFL lhs))
-           in
-              th5
-           end
-   end
-   handle HOL_ERR e => (l1 := th1; l2 := th2; raise HOL_ERR e)
+local
+   fun VALUE_RULE c = CONV_RULE (RAND_CONV (RAND_CONV c))
+   val PAIR_RULE =
+      CONV_RULE ((RATOR_CONV o RAND_CONV) (PURE_REWRITE_CONV [pairTheory.PAIR]))
+   fun ii lhs rhs =
+      let
+         val (x, y) = pairSyntax.dest_pair rhs
+         val x1 = pairSyntax.mk_fst lhs
+         val y1 = pairSyntax.mk_snd lhs
+      in
+         (x |-> x1) :: ii y1 y
+      end
+      handle HOL_ERR _ => [rhs |-> lhs]
+in
+   fun compose th1 th2 =
+      let
+         val th3 = MATCH_MP (MATCH_MP TRIPLE_COMPOSE_ALT th2) th1
+      in
+         case Thm.hyp th3 of
+            [] => th3
+          | tm :: _ =>
+              let
+                 val lemma = SYM (ASSUME tm)
+                 val (lhs, rhs) = dest_eq tm
+                 val th4 = VALUE_RULE
+                              (PairRules.UNPBETA_CONV rhs
+                               THENC REWR_CONV (SYM (SPEC_ALL LET_THM))
+                               THENC RAND_CONV (fn _ => lemma)) th3
+              in
+                 MP (PAIR_RULE (INST (ii lhs rhs) (DISCH_ALL th4))) (REFL lhs)
+              end
+      end
+      handle HOL_ERR e => (l1 := th1; l2 := th2; raise HOL_ERR e)
+end
 
 (*
 val th1 = !l1
@@ -544,108 +552,93 @@ end
   fan t
 *)
 
-val (_, mk_my_sum_case, _, _) =
-   HolKernel.syntax_fns "triple" 3
-      HolKernel.dest_triop HolKernel.mk_triop "my_sum_case"
+val case_sum_conv =
+   SIMP_CONV (std_ss++simpLib.rewrites [tripleTheory.case_sum_def]) []
+val case_sum_rule = Conv.CONV_RULE (Conv.RATOR_CONV case_sum_conv)
+val beta_fst_rule =
+   CONV_RULE ((RATOR_CONV o RAND_CONV)
+                (DEPTH_CONV PairedLambda.GEN_BETA_CONV
+                 THENC REWRITE_CONV [pairTheory.FST])
+              THENC REWRITE_CONV [boolTheory.IMP_CLAUSES])
+val forall_prod_ss = pure_ss++simpLib.rewrites [pairTheory.FORALL_PROD]
 
-fun round name (b, e) thms =
+fun round (input, get_assert, triple_refl) =
+   fn name => fn (b, e) => fn thms =>
    let
       val () = inPlaceEcho (name ^ ": ")
-      val _ = echo 1 "."
+      val () = echo 1 "."
       val t = build_compose_tree (b, e) thms
       val loop = is_rec t
-      val (_, ((th, _, _), _)) = first (fn (n, _) => (n = 0)) thms
-      val m = model (concl th)
-      val code = (concl th) |> rator |> rand
-      val pre = th |> REWRITE_RULE [wordsTheory.WORD_ADD_0]
-                   |> concl |> rator |> rator |> rand
-      val affected_vars = pre |> free_vars |> filter (fn v => not (v = !pc))
-      val input = pairSyntax.list_mk_pair affected_vars
-      fun get_assert i =
-         pairSyntax.mk_pabs (input, Term.subst (add_to_pc i) pre)
       val pre = get_assert (hd b)
       val post = get_assert (hd e)
-      val exit_th =
+      val (enter_th, exit_th) =
          if loop
-            then ISPEC m TRIPLE_REFL
-                 |> SPEC code
-                 |> SPEC (mk_my_sum_case
-                            (pre, post, sumSyntax.mk_inr (input, Type.alpha)))
-                 |> CONV_RULE (RATOR_CONV (SIMP_CONV std_ss [my_sum_case_def]))
-         else ISPEC m TRIPLE_REFL
-              |> SPEC code
-              |> SPEC (mk_comb(post,input))
-              |> CONV_RULE (RATOR_CONV (SIMP_CONV std_ss []))
-      val enter_post =
-         if loop
-            then mk_my_sum_case
-                   (pre, post, sumSyntax.mk_inl (input, Type.alpha))
-         else T
-      val enter_th =
-         if loop
-            then ISPEC m TRIPLE_REFL
-                 |> SPEC code
-                 |> SPEC enter_post
-                 |> CONV_RULE (RATOR_CONV (SIMP_CONV std_ss [my_sum_case_def]))
-         else TRUTH
+            then let
+                    fun refl_sum f =
+                       triple_refl
+                          (tripleSyntax.mk_case_sum
+                             (pre, post, f (input, Term.type_of input)))
+                 in
+                    (refl_sum sumSyntax.mk_inl, refl_sum sumSyntax.mk_inr)
+                 end
+         else (boolTheory.TRUTH, triple_refl (Term.mk_comb (post, input)))
       (* perform composition *)
-      val _ = echo 1 "."
+      val () = echo 1 "."
       fun comp (End i) = exit_th
         | comp (Repeat i) = enter_th
-        | comp (Cons (th,t)) = compose th (comp t)
-        | comp (Merge (tm,t1,t2)) = merge tm (comp t1) (comp t2)
-        | comp (ConsMerge (tm,th1,th2,t)) =
+        | comp (Cons (th, t)) = compose th (comp t)
+        | comp (Merge (tm, t1, t2)) = merge tm (comp t1) (comp t2)
+        | comp (ConsMerge (tm, th1, th2, t)) =
             let
                val res = comp t
             in
                merge tm (compose th1 res) (compose th2 res)
             end
-      val th = comp t
-      val th = th |> CONV_RULE
-                       ((RAND_CONV o RAND_CONV) (PairRules.UNPBETA_CONV input))
+      val th =
+         CONV_RULE ((RAND_CONV o RAND_CONV) (PairRules.UNPBETA_CONV input))
+            (comp t)
       val th =
          if loop
-           then let
-                   val _ = echo 1 "."
-                   (* apply loop rule *)
-                   val lemma = mk_comb (pre, input)
-                               |> SIMP_CONV std_ss [my_sum_case_def]
-                   val th =
-                      th |> CONV_RULE
-                              ((RATOR_CONV o RATOR_CONV o RAND_CONV)
-                                  (fn _ => GSYM lemma))
-                   val x = mk_var ("x", type_of input)
-                   val tm = mk_forall (x, concl th |> subst [input |-> x])
-                   val lemma = prove(tm,
-                     FULL_SIMP_TAC pure_ss [pairTheory.FORALL_PROD]
-                     THEN REPEAT STRIP_TAC
-                     THEN MATCH_MP_TAC (DISCH T th)
-                     THEN FULL_SIMP_TAC std_ss [])
-                   val th = MATCH_MP SHORT_TERM_TAILREC lemma
-                            |> CONV_RULE ((RATOR_CONV o RAND_CONV) EVAL
-                                          THENC SIMP_CONV std_ss [])
-                            |> SPEC input
-                            |> CONV_RULE ((RATOR_CONV o RATOR_CONV o RAND_CONV)
-                                             (PairRules.PBETA_CONV))
-                in
-                   th
-                end
+            then let
+                    val () = echo 1 "."
+                    (* apply loop rule *)
+                    val lemma = case_sum_conv (mk_comb (pre, input))
+                    val th = CONV_RULE ((RATOR_CONV o RATOR_CONV o RAND_CONV)
+                                           (fn _ => GSYM lemma)) th
+                    val x = Term.mk_var ("x", Term.type_of input)
+                    val tm = mk_forall (x, subst [input |-> x] (Thm.concl th))
+                    val lemma =
+                       prove
+                         (tm,
+                          FULL_SIMP_TAC forall_prod_ss []
+                          THEN REPEAT STRIP_TAC
+                          THEN MATCH_MP_TAC (DISCH T th)
+                          THEN FULL_SIMP_TAC std_ss [])
+                    val th =
+                       MATCH_MP SHORT_TERM_TAILREC lemma
+                       |> beta_fst_rule
+                       |> SPEC input
+                       |> CONV_RULE ((RATOR_CONV o RATOR_CONV o RAND_CONV)
+                                         PairRules.PBETA_CONV)
+                 in
+                    th
+                 end
          else th
-      val _ = echo 1 "."
+      val () = echo 1 "."
       val ff = th |> concl |> rand |> rand |> rator
       val def =
          new_definition (name ^ "_def", mk_eq (mk_var (name, type_of ff), ff))
       val th = th |> CONV_RULE
                        ((RAND_CONV o RAND_CONV o RATOR_CONV) (fn _ => GSYM def))
       (* clean up result *)
-      val lemma = mk_eq(mk_comb (concl def |> dest_eq |> fst, input),
+      val lemma = mk_eq(mk_comb (boolSyntax.lhs (concl def), input),
                         (!swap_primes) input)
                   |> ASSUME
       val result =
          th |> CONV_RULE ((RAND_CONV o RAND_CONV) (fn _ => lemma)
                           THENC RAND_CONV PairRules.PBETA_CONV)
             |> DISCH_ALL
-      val _ = echo 1 "."
+      val () = echo 1 "."
    in
       (def, result)
    end
@@ -653,6 +646,15 @@ fun round name (b, e) thms =
 fun core_decompile name qcode =
    let
       val (thms, loops) = time (stage_12 name) qcode
+      val (_, ((th, _, _), _)) = Lib.first (fn (x, _) => x = 0) thms
+      val (model, pre, code, _) = tripleSyntax.dest_triple (Thm.concl th)
+      val (cnd, asrt) = pairSyntax.dest_pair pre
+      val affected_vars = asrt |> Term.free_vars |> filter (fn v => v <> !pc)
+      val inp = pairSyntax.list_mk_pair (cnd :: affected_vars)
+      fun get_assert i = pairSyntax.mk_pabs (inp, Term.subst (add_to_pc i) pre)
+      val refl = Thm.SPEC code (Drule.ISPEC model tripleTheory.TRIPLE_REFL)
+      fun triple_refl t = case_sum_rule (Thm.SPEC t refl)
+      val round = round (inp, get_assert, triple_refl)
       fun rounds loops thms defs =
          let
             val (b, e) = hd loops
@@ -672,7 +674,7 @@ fun core_decompile name qcode =
       val (res, defs) =
          time (fn () => rounds loops thms [] before inPlaceEcho "Finished.\n\n")
               ()
-      val _ = add_decomp name res (loops |> last |> snd |> hd)
+      val () = add_decomp name res (loops |> last |> snd |> hd)
    in
       (res, LIST_CONJ defs)
    end
